more lemmas for encoding

theories/encoding.v
@@ -1,15 +1,15 @@
 From stdpp Require Import relations.
 From Coq Require Import ssreflect.
-From ambig Require Import grammar decidability util ambiguity acyclic.
+From ambig Require Import grammar decidability util ambiguity acyclic sub_derive.
 
 Section encoding.
 
   Variable Σ N : Type.
-  Context `{EqDecision Σ}.
-  Context `{EqDecision N}.
+  Context `{!EqDecision Σ}.
+  Context `{!EqDecision N}.
 
   Variable G : grammar Σ N.
-  Context `{acyclic G}.
+  Context `{!acyclic G}.
 
   (* sat model *)
 
@@ -75,6 +75,16 @@ Section encoding.
     l ≠ [] ↔ 0 < length l.
   Admitted.
 
+  (* TODO: since the encoding has a similar shape to the proof rules for G ⊨ A ⇒ w, 
+     we can define those proof rules first using `Inductive`, and then a first-order logic
+     proposition using disjunction, and show they are equiv to the original definition.
+
+     In this way, it suffices to show two propositions both using disjunction, but one is using
+     `can_derive` and the other `_ ⊨ _ ⇒ _`, are equiv.
+
+     This approach will also simplifies the proof for `Φ_derive k (decode _ w)`, given that
+     all `can_derive` is defined as `bool_decide (_ ⊨ _ ⇒ _)`.
+  *)
   Lemma Φ_derive_spec k m :
     Φ_derive k m →
     ∀ A x δ, 0 < δ → x + δ ≤ k →
@@ -165,5 +175,371 @@ Section encoding.
     (* TODO: why this is shelved? *)
     Unshelve. done.
   Qed.
+
+  (* encoding reachable from (S, [0..k]) *)
+  Definition Φ_reach k S : formula := λ m,
+    ∀ B x δ, (* δ can be zero *) x + δ ≤ k →
+      can_reach_from m B x δ = true ↔ (
+        (B = S ∧ x = 0 ∧ δ = k) ∨
+        (∃ A φ, A ↦ unary B φ ∈ G ∧ can_reach_from m A x δ = true ∧ apply₁ φ (decode m x δ) = true) ∨
+        (∃ A B' φ δ', x + δ + δ' ≤ k ∧ A ↦ binary B B' φ ∈ G ∧ can_reach_from m A x (δ + δ') = true ∧
+          (if bool_decide (δ' = 0) then G ⊨ B' ⇒ [] else can_derive m B' (x + δ) δ' = true) ∧
+          apply₂ φ (decode m x δ) (decode m (x + δ) δ') = true) ∨
+        (∃ A B' φ δ', δ' ≤ x (* TODO *) ∧ A ↦ binary B' B φ ∈ G ∧ can_reach_from m A (x - δ') (δ' + δ) = true ∧
+          (if bool_decide (δ' = 0) then G ⊨ B' ⇒ [] else can_derive m B' (x - δ') δ' = true) ∧
+          apply₂ φ (decode m (x - δ') δ') (decode m x δ) = true)
+      ).
+
+  Lemma Φ_reach_spec k S m :
+    Φ_derive k m →
+    Φ_reach k S m →
+    ∀ B x δ, x + δ ≤ k →
+      can_reach_from m B x δ = true ↔ reachable G (S, decode m 0 k) (B, decode m x δ).
+  Proof.
+    intros HΦ' HΦ B x δ ?. rewrite -reachable_from_spec.
+    (* induction on range length *)
+    generalize dependent B.
+    generalize dependent x.
+    induction δ as [δ IHδ] using (induction_ltof1 _ (λ δ, k - δ)) => x Hk B.
+    unfold ltof in IHδ.
+    (* induction on nonterminal *)
+    have Hwf : wf (succ G) by apply acyclic_succ_wf.
+    induction B as [B IHB] using (well_founded_induction Hwf).
+    rewrite HΦ; last done.
+    split.
+    - (* -> *) 
+      intros [Hr|[Hr|[Hr|Hr]]].
+      + destruct Hr as [-> [-> ->]]. apply reachable_from_refl.
+      + destruct Hr as [A [φ [? [? ?]]]].
+        eapply reachable_from_unary; eauto.
+        apply IHB => //. eapply succ_unary; eauto.
+      + destruct Hr as [A [B' [φ [δ' [? [? [? [? ?]]]]]]]].
+        case_bool_decide; subst.
+        * eapply reachable_from_left; eauto.
+          rewrite app_nil_r. apply IHB; last naive_solver.
+          eapply succ_left; eauto.
+        * eapply reachable_from_left; eauto.
+          2: eapply Φ_derive_spec; eauto; lia.
+          rewrite decode_merge. apply IHδ => //; lia.
+      + destruct Hr as [A [B' [φ [δ' [? [? [Hr [? ?]]]]]]]].
+        case_bool_decide; subst; eapply reachable_from_right; eauto.
+        * rewrite Nat.sub_0_r Nat.add_0_l in Hr. rewrite app_nil_l.
+          apply IHB => //. eapply succ_right; eauto.
+        * have Hx : x = x - δ' + δ' by lia.
+          rewrite {2}Hx decode_merge. apply IHδ => //; lia.
+        * eapply Φ_derive_spec; eauto; lia.
+    - (* <- *)
+      inversion 1; subst.
+      + left.
+        have Hl : length (decode m 0 k) = length (decode m x δ) by congruence.
+        rewrite !decode_length in Hl.
+        split => //. lia.
+      + right; left.
+        exists A, φ. repeat split => //.
+        apply IHB => //. eapply succ_unary; eauto.
+      + right; right; left.
+        have H3' := H3.
+        apply reachable_from_spec, reachable_sublist in H3 => //.
+        have Hw2 : w2 = decode m (x + δ) (length w2). admit.
+        have Hw2l : x + δ + length w2 ≤ k. admit.
+        exists A, Br, φ, (length w2). repeat split => //.
+        * destruct w2 => /=.
+          rewrite app_nil_r in H3'. rewrite Nat.add_0_r. apply IHB => //.
+          eapply succ_left; eauto.
+          rewrite cons_length in Hw2. rewrite cons_length in Hw2l.
+          apply IHδ; [lia.. | by rewrite -decode_merge -Hw2].
+        * destruct w2 => //=.
+          eapply Φ_derive_spec; eauto. lia.
+          rewrite cons_length in Hw2. by rewrite -Hw2.
+        * by rewrite -Hw2.
+      + right; right; right.
+        have H3' := H3.
+        apply reachable_from_spec, reachable_sublist in H3 => //.
+        have Hw1 : w1 = decode m (x - length w1) (length w1). admit.
+        have Hw1l : length w1 ≤ x. admit.
+        exists A, Bl, φ, (length w1). repeat split => //.
+        * destruct w1 => /=.
+          rewrite app_nil_l in H3'. rewrite Nat.sub_0_r. apply IHB => //.
+          eapply succ_right; eauto.
+          rewrite cons_length in Hw1. rewrite cons_length in Hw1l.
+          apply IHδ; [lia.. | ].
+          have -> : Datatypes.S (length w1 + δ) = (Datatypes.S (length w1)) + δ by lia.
+          rewrite -decode_merge Nat.sub_add //.
+          by rewrite Hw1 in H3'.
+        * destruct w1 => //=.
+          eapply Φ_derive_spec; eauto. lia.
+          rewrite Nat.sub_add //. lia.
+          rewrite cons_length in Hw1. by rewrite -Hw1.
+        * by rewrite -Hw1.
+    Admitted.
+
+  (* encoding multiple derivation *)
+
+  Definition Φ_binary_derive Bl Br φ x δl δr : formula := λ m,
+    match δl, δr with
+    | 0, _ => G ⊨ Bl ⇒ [] ∧ can_derive m Br x δr = true
+    | _, 0 => can_derive m Bl x δl = true ∧ G ⊨ Br ⇒ []
+    | _, _ => can_derive m Bl x δl = true ∧ can_derive m Br (x + δl) δr = true ∧
+      apply₂ φ (decode m x δl) (decode m (x + δl) δr) = true
+    end.
+
+  Lemma Φ_binary_derive_witness k m x δl δr A Bl Br φ :
+    Φ_derive k m →
+    x + δl + δr ≤ k →
+    A ↦ binary Bl Br φ ∈ G →
+    Φ_binary_derive Bl Br φ x δl δr m ↔
+      ∃ t1 t2, root t1 = Bl ∧ root t2 = Br ∧ word t1 = decode m x δl ∧
+        (binary_tree A t1 t2) ▷ A ={G}=> decode m x (δl + δr).
+  (* Proof.
+    intros ? ? ? ? ? [Hdl [Hdr ?]].
+    eapply Φ_derive_spec in Hdl as [t1 [? [? ?]]]; eauto; try lia.
+    eapply Φ_derive_spec in Hdr as [t2 [? [? ?]]]; eauto; try lia.
+    exists t1, t2. repeat split => //.
+    have ? : decode m x δ' ++ decode m (x + δ') (δ - δ') = decode m x δ.
+    { rewrite decode_merge. by have -> : δ' + (δ - δ') = δ by lia. }
+    repeat split. simpl in *. congruence.
+    econstructor => //. naive_solver. by rewrite H9 H6.
+  Qed. *)
+  Admitted.
+
+  Definition Φ_clause_derive (α : clause Σ N) (x δ : nat) : formula := λ m,
+    match α with
+    | ε => δ = 0
+    | atom a => δ = 1 ∧ term m x = a
+    | unary A φ =>
+      match δ with
+      | 0 => G ⊨ A ⇒ []
+      | _ => can_derive m A x δ = true ∧ apply₁ φ (decode m x δ) = true
+      end
+    | binary Bl Br φ => ∃ δl δr,
+      δl + δr = δ ∧ Φ_binary_derive Bl Br φ x δl δr m
+    end.
+
+  Lemma Φ_clause_derive_witness k m x δ A α :
+    Φ_derive k m →
+    x + δ ≤ k →
+    A ↦ α ∈ G →
+    Φ_clause_derive α x δ m ↔ match α with
+      | ε => δ = 0 ∧ ε_tree A ▷ A ={G}=> decode m x δ
+      | atom a => δ = 1 ∧ term m x = a ∧ (token_tree A (a @ (line m x, col m x))) ▷ A ={G}=> decode m x δ
+      | unary B φ => ∃ t, root t = B ∧ (unary_tree A t) ▷ A ={G}=> decode m x δ
+      | binary Bl Br φ => ∃ t1 t2, root t1 = Bl ∧ root t2 = Br ∧
+        (binary_tree A t1 t2) ▷ A ={G}=> decode m x δ
+      end.
+  Admitted.
+  (* Proof.
+    intros ? ? ? ? Hd.
+    destruct α; simpl in Hd.
+    - split; first done. repeat split. naive_solver.
+      by constructor.
+    - destruct Hd as [? ?].
+      do 2 (split; first done). repeat split. naive_solver.
+      by constructor.
+    - destruct Hd as [Hd ?].
+      eapply Φ_derive_spec in Hd as [t [? [? ?]]]; eauto.
+      exists t. split; first done. repeat split => //.
+      econstructor => //. naive_solver. by rewrite H5.
+    - destruct Hd as [δ' [? Hb]].
+      eapply binary_can_derive_witness in Hb; eauto; try lia.
+      naive_solver.
+  Qed. *)
+
+  Definition Φ_multi (A : N) (x δ : nat) : formula := λ m,
+    (∃ α β, α ≠ β ∧ A ↦ α ∈ G ∧ A ↦ β ∈ G ∧
+      Φ_clause_derive α x δ m ∧ Φ_clause_derive β x δ m) ∨
+    (∃ δ₁ δ₂ Bl Br φ, δ₁ ≠ δ₂ ∧ δ₁ ≤ δ ∧ δ₂ ≤ δ ∧ A ↦ binary Bl Br φ ∈ G ∧
+      Φ_binary_derive Bl Br φ x δ₁ (δ - δ₁) m ∧
+      Φ_binary_derive Bl Br φ x δ₂ (δ - δ₂) m).
+
+  Ltac split_exist_and :=
+    repeat match goal with
+    | [ H : _ ∧ _ |- _ ] => destruct H as [? ?]
+    | [ H : ∃ _, _ ∧ _ ∧ _ |- _ ] => destruct H as [? [? [? ?]]]
+    | [ H : ∃ _, _ ∧ _ |- _ ] => destruct H as [? [? ?]]
+    | [ H : ∃ _, _ |- _ ] => destruct H as [? ?]
+    | [ H : ∃ _ _, _ ∧ _ ∧ _ |- _ ] => destruct H as [[? [? [? [? ?]]]]]
+    | [ H : ∃ _ _,  _ ∧ _ |- _ ] => destruct H as [? [? [? ?]]]
+    | [ H : ∃ _ _, _ |- _ ] => destruct H as [? [? ?]]
+    end.
+
+  Lemma root_eq {t1 t2 A w1 w2} :
+    t1 ▷ A ={G}=> w1 →
+    t2 ▷ A ={G}=> w2 →
+    root t1 = A ∧ root t2 = A.
+  Admitted.
+
+  Ltac unify_root :=
+    match goal with
+    | [ H1 : ?t1 ▷ ?A ={?G}=> _, H2 : ?t2 ▷ ?A ={?G}=> _ |- _ ] =>
+      let Hr1 := fresh in
+      let Hr2 := fresh in
+      destruct (root_eq H1 H2) as [Hr1 Hr2]; simpl in Hr1; simpl in Hr2; subst
+    end.
+
+  Lemma multi_derive_encoding_sound k m x δ A :
+    Φ_derive k m →
+    x + δ ≤ k →
+    Φ_multi A x δ m ↔ ∃ t1 t2,
+      t1 ▷ A ={G}=> decode m x δ ∧ t2 ▷ A ={G}=> decode m x δ ∧ ¬ similar t1 t2.
+  Proof.
+    intros Hd ?. split.
+    - (* -> *)
+      intros [HΦ|HΦ].
+      + destruct HΦ as [α [β [? [? [? [Hα Hβ]]]]]].
+        eapply Φ_clause_derive_witness in Hα; eauto.
+        eapply Φ_clause_derive_witness in Hβ; eauto.
+        repeat case_match.
+        all: split_exist_and.
+        all: try congruence.
+        all: eexists; eexists.
+        all: repeat match goal with
+        | [ H : ?t ▷ ?A ={?G}=> ?w |- _ ▷ ?A ={?G}=> ?w ∧ _ ] =>
+        split; [by exact H|]; clear H
+        end => //.
+        * admit.
+        * admit.
+      + destruct HΦ as [δ₁ [δ₂ [Bl [Br [φ [? [? [? [? [Hδ₁ Hδ₂]]]]]]]]]].
+        eapply Φ_binary_derive_witness in Hδ₁ as [tl1 [tr1 [? [? [Hw1 Ht1]]]]]; eauto; try lia.
+        eapply Φ_binary_derive_witness in Hδ₂ as [tl2 [tr2 [? [? [Hw2 Ht2]]]]]; eauto; try lia.
+        have Hr1 : δ₁ + (δ - δ₁) = δ by lia. rewrite Hr1 in Ht1.
+        have Hr2 : δ₂ + (δ - δ₂) = δ by lia. rewrite Hr2 in Ht2.
+        do 2 eexists. split; first by apply Ht1. split; first by apply Ht2.
+        have ? : word tl1 ≠ word tl2.
+        { rewrite Hw1 Hw2. intros ?.
+          have : length (decode m x δ₁) = length (decode m x δ₂) by congruence.
+          by rewrite !decode_length. }
+        naive_solver.
+    - (* <- *)
+      intros [t1 [t2 [Ht1 [Ht2 Hne]]]].
+      destruct t1; destruct t2; unify_root.
+      all: simpl in Hne => //.
+      + admit.
+      + left.
+        destruct Ht1 as [? [? Ht1]]. inversion Ht1; subst; clear Ht1.
+        destruct Ht2 as [? [? Ht2]]. inversion Ht2; subst; clear Ht2.
+        exists ε, (unary (root t2) φ).
+        split => //.
+        split => //.
+        split => //.
+        split.
+          eapply Φ_clause_derive_witness; eauto. admit.
+          eapply Φ_clause_derive_witness; eauto. exists t2. admit.
+      + admit. 
+      + admit. 
+      + admit. 
+      + admit. 
+      + admit. 
+      + admit. 
+      + admit. 
+      + left.
+        destruct Ht1 as [? [? Ht1]]. inversion Ht1; subst; clear Ht1.
+        destruct Ht2 as [? [? Ht2]]. inversion Ht2; subst; clear Ht2.
+        have ? : φ0 = φ. admit. subst.
+        exists (unary (root t1) φ), (unary (root t2) φ).
+        split. naive_solver.
+        split => //.
+        split => //.
+        split.
+          eapply Φ_clause_derive_witness; eauto. exists t1. admit.
+          eapply Φ_clause_derive_witness; eauto. exists t2. admit.
+      + admit. 
+      + admit.
+      + admit.
+      + admit.
+      + destruct (decide (root t1_1 = root t2_1 ∧ root t1_2 = root t2_2)) as [Hne'|Hne'].
+        * have ? : word t1_1 ≠ word t2_1 by naive_solver.
+          right.
+          destruct Ht1 as [? [? Ht1]]. inversion Ht1; subst; clear Ht1.
+          destruct Ht2 as [? [? Ht2]]. inversion Ht2; subst; clear Ht2.
+          admit.
+        * apply not_and_l in Hne' as [|].
+          all: left.
+          all: destruct Ht1 as [? [? Ht1]]. inversion Ht1; subst; clear Ht1.
+          all: destruct Ht2 as [? [? Ht2]]. inversion Ht2; subst; clear Ht2.
+          all: admit.
+  Admitted.
+
+  (* Main theorems *)
+
+  Definition Φ_amb A k : formula := λ m,
+    Φ_derive k m ∧ Φ_reach k A m ∧ ∃ H x δ, x + δ ≤ k ∧
+      can_reach_from m H x δ = true ∧ Φ_multi H x δ m.
+
+  Theorem Φ_amb_sound A k m :
+    Φ_amb A k m → derive_amb G A (decode m 0 k).
+  Admitted.
+
+  Variable error_letter : Σ.
+  Implicit Type w : sentence Σ.
+
+  Fixpoint slice w x δ : sentence Σ :=
+    match δ with
+    | 0 => []
+    | S n =>
+      match w !! x with
+      | Some tk => tk :: slice w (x + 1) n
+      | None => []
+      end
+    end.
+
+  (* TODO: why this instance cannot be found? *)
+  (* Check acyclic_derive_dec. *)
+  (* Check acyclic_reachable_dec. *)
+
+  Global Instance acyclic_derive_dec A w :
+    Decision (G ⊨ A ⇒ w).
+  Admitted.
+
+  Global Instance acyclic_reachable_dec A w H h :
+    Decision (reachable G (A, w) (H, h)).
+  Admitted.
+
+  Definition encode (w : sentence Σ) S : model := {|
+    term i :=
+      match w !! i with
+      | Some (a @ _) => a
+      | None => error_letter
+      end;
+    line i :=
+      match w !! i with
+      | Some (_ @ (x, _)) => x
+      | None => 0
+      end;
+    col i :=
+      match w !! i with
+      | Some (_ @ (_, y)) => y
+      | None => 0
+      end;
+    can_derive A x δ := bool_decide (G ⊨ A ⇒ (slice w x δ));
+    can_reach_from A x δ := bool_decide (reachable G (S, w) (A, slice w x δ));
+  |}.
+
+  Lemma reachable_sub_word A w H h :
+    reachable G (A, w) (H, h) →
+    ∃ w1 w2, w = w1 ++ h ++ w2.
+  Admitted.
+
+  Theorem Φ_amb_complete A k w :
+    length w = k →
+    derive_amb G A w →
+    ∃ m, Φ_amb A k m (* ∧ decode m 0 k = w *).
+  Proof.
+    intros Hk Hamb.
+    apply derive_amb_iff_local_amb in Hamb; eauto.
+    destruct Hamb as [H [h [Hr [t1 [t2 [Ht1 [Ht2 Hne]]]]]]].
+    exists (encode w A).
+    have HΦ : Φ_derive k (encode w A).
+    { intros ?????. simpl. rewrite !bool_decide_eq_true. admit. }
+    have HΦ' : Φ_reach k A (encode w A).
+    { intros ????. simpl. rewrite !bool_decide_eq_true. admit. }
+    split => //. split => //.
+    have Hr' := Hr.
+    apply reachable_sub_word in Hr' as [w1 [w2 Hw]].
+    exists H, (length w1), (length h).
+    have ? : length w1 + length h ≤ k by admit.
+    split => //.
+    split. rewrite bool_decide_eq_true. admit. (* slice lemma *)
+    admit. (* multi_derive_encoding complete *)
+  Admitted.
 
 End encoding.
